library/init/lean/ir/type_check.lean
@@ -1,0 +1,251 @@
+/-
+Copyright (c) 2018 Microsoft Corporation. All rights reserved.
+Released under Apache 2.0 license as described in the file LICENSE.
+Authors: Leonardo de Moura
+-/
+prelude
+import init.lean.ir.ir init.lean.ir.format init.control.combinators
+
+namespace lean
+namespace ir
+/-- Return `tt` iff `ty` is a type that may occur in signed arithmetical operations. -/
+def is_signed_arith_ty (ty : type) : bool :=
+match ty with
+| type.int16  := tt | type.int32 := tt  | type.int64 := tt
+| type.float  := tt | type.double := tt
+| type.object := tt -- big numbers
+| _ := ff
+
+/-- Return `tt` iff `ty` is a type that may occur in arithmetical operations. -/
+def is_arith_ty (ty : type) : bool :=
+ty ≠ type.bool -- Recall that type.object may be encoding a big num.
+
+/-- Return `tt` iff `ty` is a type that may occur in non floating point arithmetical operations. -/
+def is_nonfloat_arith_ty (ty : type) : bool :=
+is_arith_ty ty && ty ≠ type.float && ty ≠ type.double
+
+/-- Return `tt` iff `ty` is a type that may occur in bitwise/logical operations. -/
+def is_bitwise_ty (ty : type) : bool :=
+match ty with
+| type.bool   := tt | type.byte := tt
+| type.uint16 := tt | type.uint32 := tt | type.uint64 := tt | type.usize := tt
+| type.object := tt
+| _ := ff
+
+/-- Return `tt` iff `ty` is a type that may occur in bitshift operations. -/
+def is_bitshift_ty (ty : type) : bool :=
+match ty with
+| type.byte   := tt
+| type.int16  := tt | type.int32 := tt  | type.int64  := tt
+| type.uint16 := tt | type.uint32 := tt | type.uint64 := tt | type.usize := tt
+| _ := ff
+
+/-- Return `tt` iff the instruction `x : r := op y` is type correct where `y : t` -/
+def valid_unop_types (op : unop) (r : type) (t : type) : bool :=
+match op with
+| unop.not          := t = r && is_bitwise_ty t
+| unop.neg          := t = r && is_signed_arith_ty t
+| unop.scalar       := t = type.object && r = type.bool
+| unop.shared       := t = type.object && r = type.bool
+| unop.copy_array   := t = type.object && r = type.object
+| unop.copy_sarray  := t = type.object && r = type.object
+| unop.box          := t ≠ type.object && r = type.object
+| unop.unbox        := t = type.object && r ≠ type.object
+| unop.unbox_bignum := t = type.object && (r = type.uint32 || r = type.int32)
+| unop.box_bignum   := r = type.object && (t = type.uint32 || t = type.int32)
+| unop.cast         := r ≠ type.object && r ≠ type.object
+
+/-- Return `tt` iff the instruction `x : r := op y z` is type correct where `y z : t` -/
+def valid_binop_types (op : binop) (r : type) (t₁ t₂ : type) : bool :=
+match op with
+| binop.add  := r = t₁ && r = t₂ && is_arith_ty r
+| binop.sub  := r = t₁ && r = t₂ && is_arith_ty r
+| binop.mul  := r = t₁ && r = t₂ && is_arith_ty r
+| binop.div  := r = t₁ && r = t₂ && is_arith_ty r
+| binop.mod  := r = t₁ && r = t₂ && is_nonfloat_arith_ty r
+| binop.shl  := r = t₁ && r = t₂ && is_bitshift_ty r
+| binop.shr  := r = t₁ && r = t₂ && is_bitshift_ty r
+| binop.ashr := r = t₁ && r = t₂ && is_bitshift_ty r
+| binop.and  := r = t₁ && r = t₂ && is_bitwise_ty r
+| binop.or   := r = t₁ && r = t₂ && is_bitwise_ty r
+| binop.xor  := r = t₁ && r = t₂ && is_bitwise_ty r
+| binop.le   := r = type.bool && t₁ = t₂ && is_arith_ty t₁
+| binop.ge   := r = type.bool && t₁ = t₂ && is_arith_ty t₁
+| binop.lt   := r = type.bool && t₁ = t₂ && is_arith_ty t₁
+| binop.gt   := r = type.bool && t₁ = t₂ && is_arith_ty t₁
+| binop.eq   := r = type.bool && t₁ = t₂
+| binop.ne   := r = type.bool && t₁ = t₂
+
+@[reducible] def type_checker_m := except_t format (reader_t (environment × list result) (state_t context id))
+
+def match_type (x : var) (t expected : type) : type_checker_m unit :=
+unless (t = expected) $
+  throw ("type mismatch, variable `" ++ to_fmt x ++ "` has type `" ++ to_fmt t ++ "`" ++
+         ", but is expected to have type `" ++ to_fmt expected ++ "`")
+
+def get_type (x : var) : type_checker_m type :=
+do m ← get,
+   match m.find x with
+   | some t := return t
+   | none   := throw ("undefined variable `" ++ to_fmt x ++ "`")
+
+def set_type (x : var) (t : type) : type_checker_m unit :=
+do m ← get,
+   match m.find x with
+   | some t' := match_type x t' t
+   | none    := put (m.insert x t)
+
+def check_type (x : var) (t : type) : type_checker_m unit :=
+do m ← get,
+   match m.find x with
+   | some t' := match_type x t' t
+   | none    := throw ("type for variable `" ++ to_fmt x ++ "` is not available")
+
+def check_ne_type (x : var) (t : type) : type_checker_m unit :=
+do m ← get,
+   match m.find x with
+   | some t' := unless (t' ≠ t) $ throw ("variable `" ++ to_fmt x ++ "` must not have type `" ++ to_fmt t ++ "`")
+   | none    := throw ("type for variable `" ++ to_fmt x ++ "` is not available")
+
+def invalid_literal : type_checker_m unit :=
+throw "invalid literal"
+
+def literal.check (l : literal) (t : type) : type_checker_m unit :=
+match l with
+| literal.bool _  := unless (t = type.bool) invalid_literal
+| literal.str  _  := unless (t = type.object) invalid_literal
+| literal.num  v  := unless (is_nonfloat_arith_ty t) invalid_literal >>
+                     when (v < 0) (unless (is_signed_arith_ty t) invalid_literal)
+| literal.float _ := unless (t = type.float || t = type.double) invalid_literal
+
+def get_decl (f : fnid) : type_checker_m decl :=
+do (env, _) ← read,
+   match env f with
+   | some d := return d
+   | none   := throw ("unknown function `" ++ to_fmt f ++ "`")
+
+def set_result_types : list var → list result → type_checker_m unit
+| []      []      := return ()
+| (x::xs) (t::ts) := set_type x t.ty >> set_result_types xs ts
+| _       _       := throw "unexpected number of return values"
+
+def instr.infer_types_core : instr → type_checker_m unit
+| (instr.lit x t l)        := set_type x t
+| (instr.unop x t op y)    := set_type x t
+| (instr.binop x t op y z) := set_type x t
+| (instr.call xs f ys)     := do d ← get_decl f, set_result_types xs d.header.return
+| (instr.cnstr o _ _ _)    := set_type o type.object
+| (instr.get x o _)        := set_type x type.object
+| (instr.sget x t o _)     := set_type x t
+| (instr.closure x f ys)   := set_type x type.object
+| (instr.apply x ys)       := set_type x type.object
+| (instr.array a sz c)     := set_type a type.object
+| (instr.read x a i)       := set_type x type.object
+| (instr.sarray a t sz c)  := set_type a type.object
+| (instr.sread x t a i)    := set_type x t
+| other                    := return ()
+
+def instr.decorate (ins : instr) (err : format) : type_checker_m unit :=
+throw $ "at instruction `" ++ to_fmt ins ++ "`" ++ format.line ++ err
+
+def instr.infer_types (ins : instr) : type_checker_m unit :=
+catch ins.infer_types_core ins.decorate
+
+def phi.decorate (p : phi) (err : format) : type_checker_m unit :=
+throw $ "at phi node `" ++ to_fmt p ++ "`" ++ format.line ++ err
+
+def phi.infer_types (p : phi) : type_checker_m unit :=
+catch (set_type p.x p.ty) p.decorate
+
+def arg.infer_types (a : arg) : type_checker_m unit :=
+set_type a.n a.ty
+
+def block.decorate (b : block) (err : format) : type_checker_m unit :=
+throw $ "at basic block `" ++ to_fmt b.id ++ "`" ++ format.line ++ err
+
+def block.infer_types (b : block) : type_checker_m unit :=
+catch (b.phis.mmap' phi.infer_types >> b.instrs.mmap' instr.infer_types) b.decorate
+
+def header.decorate {α : Type} (h : header) (err : format) : type_checker_m α :=
+throw $ "error at declaration `" ++ to_fmt h.n ++ "`" ++ format.line ++ err
+
+def decl.infer_types : decl → type_checker_m context
+| (decl.defn h bs) :=
+  catch (h.args.mmap' arg.infer_types >> bs.mmap' block.infer_types >> get) h.decorate
+| _                := get
+
+/-- Return context with the type of variables used in the given declaration.
+    It does not check whether instructions are being used correctly. -/
+def infer_types (d : decl) (env : environment) : except format context :=
+let (r, _) := (d.infer_types.run.run (env, d.header.return)).run mk_context
+in r
+
+def check_arg_types : list var → list arg → type_checker_m unit
+| []      []      := return ()
+| (x::xs) (t::ts) := check_type x t.ty >> check_arg_types xs ts
+| _       _       := throw "unexpected number of arguments"
+
+/-- Check whether the given instruction is type correct or not. It assumes the context already contains
+    the type of all variables. -/
+def instr.check_core : instr → type_checker_m unit
+| (instr.lit x t l)        := l.check t
+| (instr.unop x t op y)    := do t₁ ← get_type y, unless (valid_unop_types op t t₁) $ throw "invalid unary operation"
+| (instr.binop x t op y z) := do t₁ ← get_type y, t₂ ← get_type z, unless (valid_binop_types op t t₁ t₂) $ throw "invalid binary operation"
+| (instr.call xs f ys)     := do d ← get_decl f, check_arg_types ys d.header.args
+| (instr.cnstr o _ _ _)    := return ()
+| (instr.set o _ x)        := check_type o type.object >> check_type x type.object
+| (instr.get x o _)        := check_type o type.object
+| (instr.sset o _ x)       := check_type o type.object >> check_ne_type x type.object
+| (instr.sget x t o _)     := check_type o type.object >> check_ne_type x type.object
+| (instr.closure x f ys)   := do ys.mmap' (flip check_type type.object), d ← get_decl f,
+                                 unless (d.header.return.length = 1) $ throw "unexpected number of return values",
+                                 unless (d.header.args.length = ys.length) $ throw "unexpected number of arguments",
+                                 d.header.args.mmap' (λ a, unless (a.ty = type.object) $ throw "invalid closure, arguments must have type object")
+| (instr.apply x ys)       := ys.mmap' (flip check_type type.object)
+| (instr.array a sz c)     := check_type sz type.usize >> check_type c type.usize
+| (instr.write a i v)      := check_type a type.object >> check_type i type.usize >> check_type v type.object
+| (instr.read x a i)       := check_type a type.object >> check_type i type.usize
+| (instr.sarray a t sz c)  := check_type sz type.usize >> check_type c type.usize >> unless (t ≠ type.object) (throw "invalid scalar array")
+| (instr.swrite a i v)     := check_type a type.object >> check_type i type.usize >> check_ne_type v type.object
+| (instr.sread x t a i)    := check_ne_type x type.object >> check_type a type.object >> check_type a type.usize
+| (instr.inc x)            := check_type x type.object
+| (instr.decs x)           := check_type x type.object
+| (instr.free x)           := check_type x type.object
+| (instr.dec x)            := check_type x type.object
+
+def instr.check (ins : instr) : type_checker_m unit :=
+catch ins.check_core ins.decorate
+
+def phi.check (p : phi) : type_checker_m unit :=
+catch (p.ys.mmap' (flip check_type p.ty)) p.decorate
+
+def check_result_types : list var → list result → type_checker_m unit
+| []      []      := return ()
+| (x::xs) (t::ts) := check_type x t.ty >> check_result_types xs ts
+| _       _       := throw "unexpected number of return values"
+
+def terminator.decorate (term : terminator) (err : format) : type_checker_m unit :=
+throw $ "error at terminator `" ++ to_fmt term ++ "`" ++ format.line ++ err
+
+def terminator.check_core : terminator → type_checker_m unit
+| (terminator.ret ys)   := do (_, rs) ← read, check_result_types ys rs
+| (terminator.case x _) := do t ← get_type x, unless (t = type.object || t = type.bool) $ throw "variable must be an object or bool"
+| (terminator.jmp _)    := return ()
+
+def terminator.check (term : terminator) : type_checker_m unit :=
+catch (terminator.check_core term) term.decorate
+
+def block.check (b : block) : type_checker_m unit :=
+catch (b.phis.mmap' phi.check >> b.instrs.mmap' instr.check >> b.term.check) b.decorate
+
+def decl.check : decl → type_checker_m unit
+| (decl.defn h bs) := catch (bs.mmap' block.check) h.decorate
+| _                := return ()
+
+def type_check (d : decl) (env : environment := λ _, none) : except format context :=
+let act := do ctx ← d.infer_types, d.check, return ctx in
+let (r, _) := (act.run.run (env, d.header.return)).run mk_context in
+r
+
+end ir
+end lean
